src/functional/TreeSort.dfy
@@ -2,7 +2,7 @@ include "./BST.dfy"
 include "./List.dfy"
 
 function method TreeSort(list:List<int>, tree:BST<T>) : (sortedList:List<int>)
-  // Lemma_TreeSortListIsOrdered(list) ==> ensures list_is_ordered(TreeSort(list, Leaf))
+  // Lemma_TreeSortListIsOrdered(list, tree) ==> ensures list_is_ordered(TreeSort(list, Leaf))
   decreases list
 {
   match list {
@@ -10,3 +10,64 @@ function method TreeSort(list:List<int>, tree:BST<T>) : (sortedList:List<int>)
     case List_Empty => BST_InOrder(tree)
   }
 }
+
+/*
+lemma {:induction list} Lemma_TreeSortListIsOrdered(list:List<T>, tree:BST<T>)
+  ensures list_is_ordered(TreeSort(list, tree))
+{
+  match list {
+    case List_Empty =>
+      calc == {
+        list_is_ordered(TreeSort(list, Leaf));
+          { assert list == List_Empty; }
+        list_is_ordered(TreeSort(List_Empty, Leaf));
+          { assert TreeSort(List_Empty, Leaf) == BST_InOrder(Leaf); }
+        list_is_ordered(BST_InOrder(Leaf));
+          { assert BST_InOrder(Leaf) == List_Empty; }
+        list_is_ordered(List_Empty);
+          { assert list_is_ordered(List_Empty) == true; }
+        true;
+      }
+    case Cons(head, tail) =>
+      calc == {
+        list_is_ordered(TreeSort(list, Leaf));
+          { assert list == Cons(head, tail); }
+        list_is_ordered(TreeSort(Cons(head, tail), Leaf));
+          { assert TreeSort(Cons(head, tail), Leaf) == TreeSort(tail, BST_Insert(Leaf, head)); }
+        list_is_ordered(TreeSort(tail, BST_Insert(Leaf, head)));
+          { Lemma_InsertOrdered(tree, head); }
+          { assert BST_Insert(Leaf, head) == Node(Leaf, head, Leaf); }
+        list_is_ordered(TreeSort(tail, Node(Leaf, head, Leaf)));
+        match tail {
+          case List_Empty =>
+            calc == {
+              list_is_ordered(TreeSort(tail, Node(Leaf, head, Leaf)));
+                { assert tail == List_Empty; }
+              list_is_ordered(TreeSort(List_Empty, Node(Leaf, head, Leaf)));
+                { assert TreeSort(List_Empty, Node(Leaf, head, Leaf)) == BST_InOrder(Node(Leaf, head, Leaf)); }
+              list_is_ordered(BST_InOrder(Node(Leaf, head, Leaf)));
+                { assert BST_InOrder(Node(Leaf, head, Leaf)) == List_Concat(BST_InOrder(Leaf), Cons(head, BST_InOrder(Leaf))); }
+              list_is_ordered(List_Concat(BST_InOrder(Leaf), Cons(head, BST_InOrder(Leaf))));
+                { assert BST_InOrder(Leaf) == List_Empty; }
+              list_is_ordered(List_Concat(List_Empty, Cons(head, List_Empty)));
+                { Lemma_ConcatFirstListEmpty(List_Empty, Cons(head, List_Empty)); }
+              list_is_ordered(Cons(head, List_Empty));
+                { assert list_is_ordered(Cons(head, List_Empty)) == true; }
+              true;
+            }
+          case Cons(tah, tat) =>
+            calc == {
+              list_is_ordered(TreeSort(tail, Node(Leaf, head, Leaf)));
+                { assert tail == Cons(tah, tat); }
+              list_is_ordered(TreeSort(Cons(tah, tat), Node(Leaf, head, Leaf)));
+                { assert TreeSort(Cons(tah, tat), Node(Leaf, head, Leaf)) == TreeSort(tat, BST_Insert(Node(Leaf, head, Leaf), tah)); }
+              list_is_ordered(TreeSort(tat, BST_Insert(Node(Leaf, head, Leaf), tah)));
+                { Lemma_TreeSortListIsOrdered(tat, BST_Insert(Node(Leaf, head, Leaf), tah)); }
+              true;
+            }
+        }
+        true;
+      }
+  }
+}
+*/
